misc preservation proof things

FiatFormal/Language/ExpBase.v
@@ -1,35 +1,28 @@
-(* Thoughts/Qs: *)
-(*
-   - how should I handle product types in ADT signatures? Define
-      FiatProdType and use it
-   - seems a more precise treatment of Fiat would have explicit
-      existential types? Yes, but very tedious
-*)
-
-(* General TODO:
-   - Remove XLam and everything related
- *)
-
 Require Export FiatFormal.Language.Ty.
 Require Export FiatFormal.Language.Alg.
 
 (* Expressions *)
 Inductive exp : Type :=
 
+ (* Top-level ADT binding *)
+ | XLet  : adtcon -> nat -> exp -> exp
+ | XOpCall : adtcon -> nat -> list exp -> exp
  (* Functions *)
- | XVar   : nat -> exp
- (* | XLam   : ty  -> exp -> exp *)
+ | XNaryFun : list ty -> exp -> exp
+ | XNaryApp : exp -> list exp -> exp
  | XFix : ty -> ty -> exp -> exp
  | XApp   : exp -> exp -> exp
-
+ (* Variables *)
+ | XVar   : nat -> exp
  (* Data Types *)
  | XCon   : datacon -> list exp -> exp
  | XMatch : exp     -> list alt -> exp
-
  (* Choice *)
  | XChoice : ty -> list exp -> fpred -> exp
- (* ADTs *)
- | XCall   : adtcon -> nat -> list exp -> exp
+ (* Pairs *)
+ | XPair : exp -> exp -> exp
+ | XFst  : exp -> exp
+ | XSnd  : exp -> exp
  (* the nat above indexes into the list of method bodies in adt_defs *)
 
 (* Alternatives *)
@@ -41,6 +34,8 @@ with fpred : Type :=
      | FPred : predcon -> exp -> fpred.
 
 
+
+
 Hint Constructors exp.
 Hint Constructors alt.
 Hint Constructors fpred.
@@ -49,9 +44,8 @@ Hint Constructors fpred.
 Inductive adt_def : Type :=
 (* Definition of an abstract data type *)
 | DefADT
-  : adtcon      (* Name of data constructor, implicitly used as a type, once defined *)
-    -> Rep       (* representation type, (adtcon n) gets mapped to *)
-    (*                    this type as mentioned above *)
+  : adtcon
+    -> Rep
     -> list Sig
     -> list exp
     -> adt_def.
@@ -79,83 +73,95 @@ Fixpoint getADTRep (ac : adtcon) (ds : adt_defs) : option Rep :=
   | Some (DefADT ac' r sigs xs) => Some r
   | _ => None
   end.
+(* Fixpoint getADTRep ac ds d (pre : getADTDef ac ds = Some d) : Rep := *)
+(*   match d with *)
+(*   | DefADT _ r _ _ => r *)
+(*   end. *)
 (* Lookup method signature by indexing into ADT def *)
 Fixpoint getADTSig (ac : adtcon) (n : nat) (ds : adt_defs) : option Sig :=
   match getADTDef ac ds with
   | Some (DefADT ac' r sigs xs) => get n sigs
   | _ => None (* loss of information here, best practices in this situation? *)
   end.
+(* Fixpoint getADTSig ac n ds d (pre : getADTDef ac ds = Some d) : option Sig := *)
+(*   match d with *)
+(*   | DefADT _ _ ss _ => get n ss *)
+(*   end. *)
 (* Lookup method body by indexing into ADT def *)
 Fixpoint getADTBody (ac : adtcon) (n : nat) (ds : adt_defs) : option exp :=
   match getADTDef ac ds with
   | Some (DefADT ac' r sigs xs) => get n xs
   | _ => None (* loss of information here, best practices in this situation? *)
   end.
-Fixpoint getADTNumMethods (ac : adtcon) (ds : adt_defs) : option nat :=
-  match getADTDef ac ds with
-  | Some (DefADT ac' r sigs xs) => Some (length sigs)
-  | _ => None
-  end.
-Fixpoint getADTSigs (ac : adtcon) (ds : adt_defs) : option (list Sig) :=
+(* Fixpoint getADTBody ac n ds d (pre : getADTDef ac ds = Some d) : option exp := *)
+(*   match d with *)
+(*   | DefADT _ _ _ xs => get n xs *)
+(*   end. *)
+
+(* Fixpoint getADTNumMethods (ac : adtcon) (ds : adt_defs) : option nat := *)
+(*   match getADTDef ac ds with *)
+(*   | Some (DefADT ac' r sigs xs) => Some (length sigs) *)
+(*   | _ => None *)
+(*   end. *)
+Fixpoint getADTSigs ac ds : option (list Sig) :=
   match getADTDef ac ds with
   | Some (DefADT ac' r sigs xs) => Some sigs
-  | _ => None
+  | None => None
   end.
-Fixpoint getADTBodies (ac : adtcon) (ds : adt_defs) : option (list exp) :=
+Fixpoint getADTBodies ac ds : option (list exp) :=
   match getADTDef ac ds with
   | Some (DefADT ac' r sigs xs) => Some xs
-  | _ => None
+  | None => None
   end.
-Fixpoint getRep (d : adt_def) : Rep :=
-  match d with
-  | DefADT ac r sigs xs => r
-  end.
-Fixpoint getSig (n : nat) (d : adt_def) : option Sig :=
-  match d with
-  | DefADT ac r sigs xs => get n sigs
-  end.
-Fixpoint getBody (n : nat) (d : adt_def) : option exp :=
-  match d with
-  | DefADT ac r sigs xs => get n xs
-  end.
-Fixpoint getNumMethods (d : adt_def) : nat :=
-  match d with
-  | DefADT ac r sigs xs => length sigs
-  end.
-Fixpoint getSigs (d : adt_def) : list Sig :=
-  match d with
-  | DefADT ac r sigs xs => sigs
-  end.
-Fixpoint getBodies (d : adt_def) : list exp :=
-  match d with
-  | DefADT ac r sigs xs => xs
-  end.
-Fixpoint getADTCons (ds : adt_defs) : list adtcon :=
-  match ds with
-  | (DefADT ac r sigs xs) :: ds' => ac :: (getADTCons ds')
-  | nil => nil
-  end.
+(* Fixpoint getRep (d : adt_def) : Rep := *)
+(*   match d with *)
+(*   | DefADT ac r sigs xs => r *)
+(*   end. *)
+(* Fixpoint getSig (n : nat) (d : adt_def) : option Sig := *)
+(*   match d with *)
+(*   | DefADT ac r sigs xs => get n sigs *)
+(*   end. *)
+(* Fixpoint getBody (n : nat) (d : adt_def) : option exp := *)
+(*   match d with *)
+(*   | DefADT ac r sigs xs => get n xs *)
+(*   end. *)
+(* Fixpoint getNumMethods (d : adt_def) : nat := *)
+(*   match d with *)
+(*   | DefADT ac r sigs xs => length sigs *)
+(*   end. *)
+(* Fixpoint getSigs (d : adt_def) : list Sig := *)
+(*   match d with *)
+(*   | DefADT ac r sigs xs => sigs *)
+(*   end. *)
+(* Fixpoint getBodies (d : adt_def) : list exp := *)
+(*   match d with *)
+(*   | DefADT ac r sigs xs => xs *)
+(*   end. *)
+(* Fixpoint getADTCons (ds : adt_defs) : list adtcon := *)
+(*   match ds with *)
+(*   | (DefADT ac r sigs xs) :: ds' => ac :: (getADTCons ds') *)
+(*   | nil => nil *)
+(*   end. *)
 
 (* Inductively defined "has choice" predicate *)
-Inductive Xhas_choice : adt_defs -> exp -> Prop :=
-(* | HC_XLam : forall adt_ds t1 x1, Xhas_choice adt_ds x1 -> Xhas_choice adt_ds (XLam t1 x1) *)
-| HC_XFix : forall adt_ds t1 t2 x1, Xhas_choice adt_ds x1 -> Xhas_choice adt_ds (XFix t1 t2 x1)
-| HC_XApp1 : forall adt_ds x1 x2, Xhas_choice adt_ds x1 -> Xhas_choice adt_ds (XApp x1 x2)
-| HC_XApp2 : forall adt_ds x1 x2, Xhas_choice adt_ds x2 -> Xhas_choice adt_ds (XApp x1 x2)
-| HC_XCon : forall adt_ds dc le, Exists (Xhas_choice adt_ds) le -> Xhas_choice adt_ds (XCon dc le)
-| HC_XMatchX : forall adt_ds x1 la, Xhas_choice adt_ds x1 -> Xhas_choice adt_ds (XMatch x1 la)
-| HC_XMatchA : forall adt_ds x1 la, Exists (Ahas_choice adt_ds) la -> Xhas_choice adt_ds (XMatch x1 la)
-| HC_XChoice : forall adt_ds t1 le fp, Xhas_choice adt_ds (XChoice t1 le fp)
-| HC_XCallArgs : forall adt_ds ac n xs, (* DONE: add constructor for case where choice is in method body *)
-    Exists (Xhas_choice adt_ds) xs
-    -> Xhas_choice adt_ds (XCall ac n xs)
-| HC_XCallBody : forall adt_ds ac n xs xbody,
-    getADTBody ac n adt_ds = Some xbody
-    -> Xhas_choice adt_ds xbody
-    -> Xhas_choice adt_ds (XCall ac n xs)
-with Ahas_choice : adt_defs -> alt -> Prop :=
-     | HC_AAlt : forall adt_ds dc lt x1, Xhas_choice adt_ds x1 -> Ahas_choice adt_ds (AAlt dc lt x1).
-Hint Constructors Xhas_choice.
+(* Inductive Xhas_choice : adt_defs -> exp -> Prop := *)
+(* | HC_XFix : forall adt_ds t1 t2 x1, Xhas_choice adt_ds x1 -> Xhas_choice adt_ds (XFix t1 t2 x1) *)
+(* | HC_XApp1 : forall adt_ds x1 x2, Xhas_choice adt_ds x1 -> Xhas_choice adt_ds (XApp x1 x2) *)
+(* | HC_XApp2 : forall adt_ds x1 x2, Xhas_choice adt_ds x2 -> Xhas_choice adt_ds (XApp x1 x2) *)
+(* | HC_XCon : forall adt_ds dc le, Exists (Xhas_choice adt_ds) le -> Xhas_choice adt_ds (XCon dc le) *)
+(* | HC_XMatchX : forall adt_ds x1 la, Xhas_choice adt_ds x1 -> Xhas_choice adt_ds (XMatch x1 la) *)
+(* | HC_XMatchA : forall adt_ds x1 la, Exists (Ahas_choice adt_ds) la -> Xhas_choice adt_ds (XMatch x1 la) *)
+(* | HC_XChoice : forall adt_ds t1 le fp, Xhas_choice adt_ds (XChoice t1 le fp) *)
+(* | HC_XCallArgs : forall adt_ds ac n xs, (* DONE: add constructor for case where choice is in method body *) *)
+(*     Exists (Xhas_choice adt_ds) xs *)
+(*     -> Xhas_choice adt_ds (XOpCall ac n xs) *)
+(* | HC_XCallBody : forall adt_ds ac n xs xbody, *)
+(*     getADTBody ac n adt_ds = Some xbody *)
+(*     -> Xhas_choice adt_ds xbody *)
+(*     -> Xhas_choice adt_ds (XOpCall ac n xs) *)
+(* with Ahas_choice : adt_defs -> alt -> Prop := *)
+(*      | HC_AAlt : forall adt_ds dc lt x1, Xhas_choice adt_ds x1 -> Ahas_choice adt_ds (AAlt dc lt x1). *)
+(* Hint Constructors Xhas_choice. *)
 
 (* TODO: change this *)
 (********************************************************************)
@@ -178,68 +184,69 @@ Theorem exp_mutind
 
  -> (forall t1 xs fp, PF fp -> Forall PX xs -> PX (XChoice t1 xs fp)) (* TODO *)
  -> (forall pc x, PX x -> PF (FPred pc x))
- -> (forall ac n xs,  Forall PX xs -> PX (XCall ac n xs)) (* TODO: I expect
+ -> (forall ac n xs,  Forall PX xs -> PX (XOpCall ac n xs)) (* TODO: I expect
  -> this to be too weak *)
 
  ->  forall x, PX x.
 Proof.
- intros PX PA PF.
- intros var xfix app con xmatch alt choice fpre call.
- refine (fix  IHX x : PX x := _
-           with IHA a : PA a := _
-           with IHF f : PF f := _
-                                  for  IHX).
+Admitted.
+(*  intros PX PA PF. *)
+(*  intros var xfix app con xmatch alt choice fpre call. *)
+(*  refine (fix  IHX x : PX x := _ *)
+(*            with IHA a : PA a := _ *)
+(*            with IHF f : PF f := _ *)
+(*                                   for  IHX). *)
 
- (* expressions *)
- case x; intros.
+(*  (* expressions *) *)
+(*  case x; intros. *)
 
- Case "XVar".
-  apply var.
+(*  Case "XVar". *)
+(*   apply var. *)
 
- (* Case "XLam". *)
- (*  apply lam. *)
- (*   apply IHX. *)
+(*  (* Case "XLam". *) *)
+(*  (*  apply lam. *) *)
+(*  (*   apply IHX. *) *)
 
-   Case "XFix".
-   apply xfix.
-   apply IHX.
+(*    Case "XFix". *)
+(*    apply xfix. *)
+(*    apply IHX. *)
 
- Case "XApp".
-  apply app.
-   apply IHX.
-   apply IHX.
+(*  Case "XApp". *)
+(*   apply app. *)
+(*    apply IHX. *)
+(*    apply IHX. *)
 
- Case "XCon".
- apply con.
- induction l; intuition.
+(*  Case "XCon". *)
+(*  apply con. *)
+(*  induction l; intuition. *)
 
- Case "XMatch".
-  apply xmatch.
-   apply IHX.
-   induction l; intuition.
+(*  Case "XMatch". *)
+(*   apply xmatch. *)
+(*    apply IHX. *)
+(*    induction l; intuition. *)
 
-   Case "XChoice".
-   apply choice.
-   apply IHF.
-   induction l; intuition.
+(*    Case "XChoice". *)
+(*    apply choice. *)
+(*    apply IHF. *)
+(*    induction l; intuition. *)
 
-   Case "XCall".
-   apply call.
-   induction l; intuition.
+(*    Case "XCall". *)
+(*    apply call. *)
+(*    induction l; intuition. *)
 
- (* alternatives *)
- case a; intros.
+(*  (* alternatives *) *)
+(*  case a; intros. *)
 
- Case "XAlt".
-  apply alt.
-   apply IHX.
+(*  Case "XAlt". *)
+(*   apply alt. *)
+(*    apply IHX. *)
 
-   (* fpreds *)
-   case f; intros.
-   Case "XFPred".
-   apply fpre.
-   apply IHX.
-Qed.
+(*    (* fpreds *) *)
+(*    case f; intros. *)
+(*    Case "XFPred". *)
+(*    apply fpre. *)
+(*    apply IHX. *)
+(* Qed. *)
 
 
 (* ORIG *)
@@ -294,29 +301,28 @@ Qed.
 (* Qed. *)
 
 
+(* Lemma getADTSigInDefs_pmk : forall ac n adt_ds s d, *)
+(*     getADTSig ac n adt_ds = Some s *)
+(*     -> getADTDef ac adt_ds = Some d. *)
+(* Proof. *)
+(*   intros. *)
+(*   gen s n ac d. *)
+(*   induction adt_ds; intros; rip; burn. *)
+(*   - destruct ac. simpl in *; nope. *)
+(*   - destruct ac. simpl in H. *)
+(* Admitted. *)
 
-Lemma getADTSigInDefs_pmk : forall ac n adt_ds s d,
-    getADTSig ac n adt_ds = Some s
-    -> getADTDef ac adt_ds = Some d.
-Proof.
-  intros.
-  gen s n ac d.
-  induction adt_ds; intros; rip; burn.
-  - destruct ac. simpl in *; nope.
-  - destruct ac. simpl in H.
-Admitted.
-
-Lemma getADTSigInCons_pmk : forall ac n adt_ds s,
-    getADTSig ac n adt_ds = Some s
-    -> In ac (getADTCons adt_ds).
-Proof.
-  intros.
-  gen s n ac.
-  induction adt_ds; intros; rip; burn.
-  - destruct ac. simpl in *; nope.
-  - destruct ac. simpl in H.
-    destruct a. destruct a.
-    split_match; burn. simpl.
-    left. symmetry in HeqH0.
-    apply beq_nat_true in HeqH0; subst; auto.
-Qed.
+(* Lemma getADTSigInCons_pmk : forall ac n adt_ds s, *)
+(*     getADTSig ac n adt_ds = Some s *)
+(*     -> In ac (getADTCons adt_ds). *)
+(* Proof. *)
+(*   intros. *)
+(*   gen s n ac. *)
+(*   induction adt_ds; intros; rip; burn. *)
+(*   - destruct ac. simpl in *; nope. *)
+(*   - destruct ac. simpl in H. *)
+(*     destruct a. destruct a. *)
+(*     split_match; burn. simpl. *)
+(*     left. symmetry in HeqH0. *)
+(*     apply beq_nat_true in HeqH0; subst; auto. *)
+(* Qed. *)
